split

Flows/Groundwork.lean
@@ -4,8 +4,34 @@ Released under Apache 2.0 license as described in the file LICENSE.
 Authors: Julien Marquet
 -/
 
-import MyPackage.Base
-import MyPackage.Notation
+section /- Basic definitions -/
+
+class RSMul (χ α : Type u) where
+  smul : χ → α → χ
+
+class HasMem (χ α : Type u) where
+  mem : χ → α → Prop
+
+class HasUnion (α : Type u) where
+  union : α → α → α
+
+class HasIncluded (α : Type u) where
+  included : α → α → Prop
+
+class HasWithout (α : Type u) where
+  without : α → α → α
+
+class HasVehicle (α β : Type u) where
+  vehicle : α → β
+
+infix:70 " • " => RSMul.smul
+infix:50 " ∈ " => HasMem.mem
+infixl:60 " ∪ " => HasUnion.union
+infix:50 " ⊆ " => HasIncluded.included
+infixl:65 " \\ " => HasWithout.without
+notation:max "𝒱 " a:arg => HasVehicle.vehicle a
+
+end
 
 open Classical
 
