Flows/Subst.lean
@@ -1,0 +1,191 @@
+/-
+Copyright (c) 2021-2022 Julien Marquet. All rights reserved.
+Released under Apache 2.0 license as described in the file LICENSE.
+Authors: Julien Marquet
+-/
+
+import Flows.Term
+
+open Classical
+
+set_option codegen false
+
+def Subst (α : Type u) (β : Type u) := { f : β → Term α β // finite { x : β // f x ≠ Term.Var x } }
+
+private theorem comp_carrier {f g : β → Term α β} {x : β} :
+  ((f * g) x ≠ Term.Var x) → f x ≠ Term.Var x ∨ g x ≠ Term.Var x := by
+  rw [← Decidable.not_and_iff_or_not]
+  apply contrapose
+  exact λ ⟨ h₁, h₂ ⟩ => by simp [HMul.hMul, Mul.mul, comp, map_reduce, h₁, h₂]
+
+private def carriers_arrow (f g : β → Term α β) : ({ x : β // (f * g) x ≠ Term.Var x }) →
+  { x // f x ≠ Term.Var x } ⊕ { x // g x ≠ Term.Var x } :=
+  λ ⟨ x, p ⟩ =>
+    if hf : f x ≠ Term.Var x then Sum.inl ⟨ x, hf ⟩
+    else if hg : g x ≠ Term.Var x then Sum.inr ⟨ x, hg ⟩
+    else False.elim <| match comp_carrier p with
+    | Or.inl p => hf p
+    | Or.inr p => hg p
+
+private theorem carriers_arrow_inj (f g : β → Term α β) (x y : {x // (f * g) x ≠ Term.Var x})
+  (h : carriers_arrow f g x = carriers_arrow f g y) : x = y := by
+  revert x y
+  intro ⟨ x, hx ⟩ ⟨ y, hy ⟩ h
+  apply Subtype.eq
+  simp [carriers_arrow] at h
+  have x_nontriv : {P : Prop} → ¬ f x ≠ Term.Var x → ¬ g x ≠ Term.Var x → P :=
+    λ p q => False.elim <| match comp_carrier hx with | Or.inl r => p r | Or.inr r => q r
+  have y_nontriv : {P : Prop} → ¬ f y ≠ Term.Var y → ¬ g y ≠ Term.Var y → P :=
+    λ p q => False.elim <| match comp_carrier hy with | Or.inl r => p r | Or.inr r => q r
+  by_cases p₁ : f x ≠ Term.Var x <;> by_cases p₂ : g x ≠ Term.Var x
+    <;> by_cases p₃ : f y ≠ Term.Var y <;> by_cases p₄ : g y ≠ Term.Var y
+    <;> simp [dif_pos p₁, dif_neg p₁, dif_pos p₂, dif_neg p₂,
+      dif_pos p₃, dif_neg p₃, dif_pos p₄, dif_neg p₄] at h
+    <;> first
+      | assumption
+      | apply x_nontriv; assumption; assumption
+      | apply y_nontriv; assumption; assumption
+
+instance : Monoid (Subst α β) where
+  one := ⟨ Term.Var, ⟨ [], λ ⟨ _, p ⟩ => p rfl ⟩ ⟩
+  mul := λ ⟨ f, pf ⟩ ⟨ g, pg ⟩ =>
+    ⟨ f * g, invimage_finite_of_inj (sum_finite pf pg) (carriers_arrow_inj f g) ⟩
+  one_mul := λ ⟨ _, _ ⟩ => rfl
+  mul_one := λ ⟨ _, _ ⟩ => Subtype.eq <| fun_monoid.mul_one _
+  mul_assoc := λ ⟨ _, _ ⟩ ⟨ _, _ ⟩ ⟨ _, _ ⟩ => Subtype.eq <| fun_monoid.mul_assoc _ _ _
+
+instance subst_self_action : RAction (Subst α β) (Subst α β) := self_action _
+
+instance subst_term_action : RAction (Term α β) (Subst α β) where
+  smul := λ x ⟨ f, hf ⟩ => x • f
+  smul_one := term_action.smul_one
+  smul_mul := λ _ ⟨ _, _ ⟩ ⟨ _, _ ⟩ => term_action.smul_mul _ _ _
+
+def Subst.ext {θ φ : Subst α β} : θ = φ
+  ↔ ∀ x, (Term.Var x : Term α β) • θ = (Term.Var x : Term α β) • φ := by
+  apply Iff.intro (by intro h _; rw [h])
+  intro h
+  match θ with
+  | ⟨ θ, _ ⟩ => match φ with
+    | ⟨ φ, _ ⟩ =>
+      apply Subtype.eq
+      funext x
+      exact h x
+
+def Subst.elementary {x : β} {u : Term α β} (h : Term.Var x ≠ u) : Subst α β :=
+  ⟨ λ z => if z = x then u else Term.Var z, by
+    apply Exists.intro [⟨ x, by simp [h.symm] ⟩]
+    intro ⟨ z, hz ⟩
+    simp [List.mem]
+    apply byContradiction
+    intro h'
+    apply hz
+    simp [h'] ⟩
+
+theorem Subst.elementary_spec₁ {x : β} {u : Term α β} (h : Term.Var x ≠ u) :
+  (Term.Var x : Term α β) • (elementary h : Subst α β) = u := by
+  simp [RSMul.smul, elementary, map_reduce]
+
+theorem Subst.elementary_spec₂ {x z : β} {u : Term α β} (h : Term.Var x ≠ u) (h' : z ≠ x) :
+  (Term.Var z : Term α β) • (elementary h : Subst α β) = Term.Var z := by
+  simp [RSMul.smul, elementary, map_reduce, h']
+
+def carrier (θ : Subst α β) : Fintype β :=
+  match θ with
+  | ⟨ θ, h ⟩ =>
+    let π : {x // θ x ≠ Term.Var x} → β := λ ⟨ x, _ ⟩ => x
+    Fintype.mk <| List.map π (epsilon <| λ l => ∀ a, List.mem a l)
+
+def carrier_spec {θ : Subst α β} {y : β} :
+  y ∈ carrier θ ↔ (Term.Var y : Term α β) • θ ≠ Term.Var y :=
+  match θ with
+  | ⟨ θ, hθ ⟩ => by
+    apply Iff.intro
+    focus
+      intro h
+      let ⟨ ⟨ x, hx ⟩, ⟨ _, h₂ ⟩ ⟩ := List.mem_map_iff_image.1 h
+      exact h₂ ▸ hx
+    focus
+      let π : {x // θ x ≠ Term.Var x} → β := λ ⟨ x, _ ⟩ => x
+      intro h'
+      rw [show y = π ⟨ y, h' ⟩ from rfl]
+      apply List.mem_map
+      apply epsilon_spec hθ
+
+theorem is_one_iff_empty_carrier {θ : Subst α β} : θ = 1 ↔ carrier θ = ∅ := by
+  apply Iff.intro
+  focus
+    intro h
+    rw [h, Fintype.ext]
+    intro x
+    apply Iff.intro _ (False.elim ∘ Fintype.not_mem_empty _)
+    rw [carrier_spec]
+    exact λ h => False.elim <| h rfl
+  focus
+    intro h
+    rw [Subst.ext]
+    intro x
+    apply byContradiction
+    intro h'
+    apply Fintype.not_mem_empty x
+    rw [← h, carrier_spec]
+    exact h'
+
+theorem carrier_one : carrier (1 : Subst α β) = ∅ :=
+  is_one_iff_empty_carrier.1 rfl
+
+theorem is_one_iff_not_modifying (θ : Subst α β) :
+  θ = 1 ↔ ∀ x, (Term.Var x : Term α β) • θ = Term.Var x := Subst.ext
+
+theorem not_one_iff_modifying (θ : Subst α β) :
+  θ ≠ 1 ↔ ∃ x, (Term.Var x : Term α β) • θ ≠ Term.Var x := by
+  apply Iff.intro
+  focus
+    intro h
+    apply byContradiction
+    intro h'
+    apply h
+    rw [Subst.ext]
+    intro x
+    apply byContradiction
+    intro h''
+    exact h' ⟨ x, h'' ⟩
+  focus
+    intro ⟨ x, h ⟩ h'
+    rw [is_one_iff_not_modifying] at h'
+    exact h (h' x)
+
+theorem elementary_carrier {x : β} {u : Term α β} {h : Term.Var x ≠ u} :
+  carrier (Subst.elementary h : Subst α β) = Fintype.mk [x] := by
+  apply Fintype.ext.2
+  intro y
+  rw [carrier_spec]
+  apply Iff.intro
+  focus
+    by_cases p : y = x
+    focus
+      rw [p]
+      intro _
+      simp [Fintype.mem_mk_iff, List.mem]
+    focus
+      intro h'
+      apply False.elim ∘ h'
+      simp [Subst.elementary, RSMul.smul, map_reduce, p]
+  focus
+    rw [Fintype.mem_mk_iff]
+    intro p
+    rw [show y = x by simp_all [List.mem], Subst.elementary_spec₁]
+    exact Ne.symm h
+
+theorem carrier_cons (θ φ : Subst α β) : carrier (θ * φ) ⊆ carrier θ ∪ carrier φ := by
+  intro x
+  rw [Fintype.mem_union_iff]
+  simp only [carrier_spec]
+  match θ with
+  | ⟨ θ, _ ⟩ => match φ with
+    | ⟨ φ, _ ⟩ => exact comp_carrier
+
+theorem subst_cons {u v : Term α β} {θ : Subst α β} :
+  Term.Cons u v • θ = Term.Cons (u • θ) (v • θ) := by
+  cases θ; rfl
+
