Flows/Term.lean
@@ -1,0 +1,82 @@
+/-
+Copyright (c) 2021-2022 Julien Marquet. All rights reserved.
+Released under Apache 2.0 license as described in the file LICENSE.
+Authors: Julien Marquet
+-/
+
+import Lean
+
+import Flows.Groundwork
+
+open Classical
+
+set_option codegen false
+
+universe u
+
+inductive Term (α : Type u) (β : Type u)
+  | Cst (c : α)
+  | Var (x : β)
+  | Cons (t₁ : Term α β) (t₂ : Term α β)
+
+section
+
+variable {α : Type u} {β : Type u}
+
+def map_reduce (θ : β → Term α β) (u : Term α β) : Term α β := match u with
+  | Term.Cst c => Term.Cst c
+  | Term.Var x => θ x
+  | Term.Cons t₁ t₂ => Term.Cons (map_reduce θ t₁) (map_reduce θ t₂)
+
+def comp (f g : β → Term α β) (x : β) : Term α β :=
+  map_reduce g (f x)
+
+theorem map_one (u : Term α β) : map_reduce Term.Var u = u :=
+  by induction u with
+  | Cst c => rfl
+  | Var x => rfl
+  | Cons t₁ t₂ ht₁ ht₂ => simp [map_reduce, ht₁, ht₂]
+
+theorem map_comp (u : Term α β) (f g : β → Term α β) :
+  map_reduce g (map_reduce f u) = map_reduce (comp f g) u := by induction u with
+  | Cst c => rfl
+  | Var x => rfl
+  | Cons t₁ t₂ ht₁ ht₂ => simp [map_reduce, ht₁, ht₂]
+
+instance fun_monoid : Monoid (β → Term α β) where
+  one := Term.Var
+  mul := comp
+  one_mul := by intros; rfl
+  mul_one := by intros; funext x; apply map_one
+  mul_assoc := by intros; funext x; apply map_comp
+
+instance term_action : RAction (Term α β) (β → Term α β) where
+  smul x θ := map_reduce θ x
+  smul_one := map_one
+  smul_mul := map_comp
+
+end
+
+section
+
+variable {α β : Type u}
+
+def mass : (u : Term α β) → Nat
+| Term.Cst _ => 0
+| Term.Var _ => 0
+| Term.Cons l r => mass l + mass r + 1
+
+theorem mass_decr_l (l r : Term β α) : mass l < mass (Term.Cons l r) :=
+  Nat.lt_succ_of_le <| Nat.le_add_right _ _
+
+theorem mass_decr_r (l r : Term β α) : mass r < mass (Term.Cons l r) :=
+  Nat.lt_succ_of_le <| Nat.le_add_left _ _
+
+def Term.mass_wfRel : WellFoundedRelation (Term α β) := measure mass
+
+def weight (x : β) : (u : Term α β) → Nat
+| Term.Cst _ => 0
+| Term.Var y => if x = y then 1 else 0
+| Term.Cons l r => weight x l + weight x r
+
+end
