Flows/Unifier.lean
@@ -1,0 +1,66 @@
+/-
+Copyright (c) 2021-2022 Julien Marquet. All rights reserved.
+Released under Apache 2.0 license as described in the file LICENSE.
+Authors: Julien Marquet
+-/
+
+import Flows.Term
+import Flows.Subst
+
+open Classical
+
+set_option codegen false
+
+section
+
+variable {χ : Type u} (α : Type u) [Monoid α] [RAction χ α]
+
+def unifiers (a b : χ) := λ (θ : α) => a • θ = b • θ
+
+def generated_by (θ : α) := λ (φ : α) => ∃ ρ, θ * ρ = φ
+
+def is_mgu (a b : χ) (θ : α) := unifiers α a b = generated_by α θ
+def strangers (a b : χ) := unifiers α a b = λ _ => False
+
+def mgu_or_strangers (a b : χ) :=
+  (∃ θ : α, unifiers α a b = generated_by α θ) ∨ strangers α a b
+
+end
+
+section
+
+variable {χ : Type u} {α : Type u} [Monoid α] [RAction χ α]
+
+theorem unifies_of_mgu {u v : χ} {θ : α} (h : is_mgu α u v θ) : u • θ = v • θ := by
+  suffices unifiers _ _ _ _ by assumption
+  exact h ▸ Exists.intro 1 (Monoid.mul_one _)
+
+theorem most_general_of_mgu {a b : χ} {θ φ : α}
+  (h₁ : is_mgu α a b θ) (h₂ : a • φ = b • φ) : ∃ ρ, θ * ρ = φ := by
+  suffices generated_by α θ φ by assumption
+  exact h₁ ▸ h₂
+
+theorem mgu_of_unifies_and_most_general {a b : χ} {θ : α}
+  (unifies : a • θ = b • θ)
+  (most_general : ∀ φ, a • φ = b • φ → ∃ ρ, θ * ρ = φ) : is_mgu α a b θ := by
+  funext φ
+  apply propext
+  apply Iff.intro (most_general _)
+  intro ⟨ ρ, hρ ⟩
+  rw [← hρ, ← RAction.smul_mul, ← RAction.smul_mul, unifies]
+
+theorem strangers_iff_no_unifier {u v : χ} :
+  strangers α u v ↔ ∀ θ : α, u • θ ≠ v • θ := by
+  apply Iff.intro
+  focus
+    intro h θ h'
+    suffices p : unifiers α u v θ by
+      rw [h] at p; exact False.elim p
+    exact h'
+  focus
+    intro h
+    funext θ
+    apply propext
+    apply Iff.intro (λ h' => h θ h') (λ h => False.elim h)
+
+end
