Flows/Vanishing.lean
@@ -1,0 +1,108 @@
+/-
+Copyright (c) 2021-2022 Julien Marquet. All rights reserved.
+Released under Apache 2.0 license as described in the file LICENSE.
+Authors: Julien Marquet
+-/
+
+import Flows.Groundwork
+import Flows.Term
+import Flows.Subst
+import Flows.Vehicle
+
+open Classical
+
+set_option codegen false
+
+section
+
+variable {α β : Type u}
+
+def vanishing (θ : Subst α β) :=
+  ∀ {x}, (Term.Var x : Term α β) • θ ≠ Term.Var x →
+    ∀ y, ¬ (x ∈ (𝒱 ((Term.Var y : Term α β) • θ) : Fintype β))
+
+theorem vanishing_on_term {θ : Subst α β} (h₁ : vanishing θ)
+  {x : β} (h₂ : (Term.Var x : Term α β) • θ ≠ Term.Var x)
+  (u : Term α β) : ¬ x ∈ (𝒱 (u • θ) : Fintype β) := by
+  induction u with
+  | Cst c => match θ with
+    | ⟨ θ, h ⟩ => intro h; exact h
+  | Var y => exact h₁ h₂ _
+  | Cons l r hl hr =>
+    rw [subst_cons]
+    intro h
+    cases (Fintype.mem_union_iff _ _ _).1 h with
+    | inl h => exact hl h
+    | inr h => exact hr h
+
+theorem vanishing_on_vehicle {θ : Subst α β} (h₁ : vanishing θ)
+  {x : β} (h₂ : (Term.Var x : Term α β) • θ ≠ Term.Var x) :
+  ¬ x ∈ (𝒱 θ : Fintype β) := by
+  suffices h : 𝒱 θ ⊆ 𝒱 θ \ (Fintype.mk [x]) by
+    apply Fintype.not_mem_iff_in_without.2
+    exact h
+  conv => lhs; simp only [HasVehicle.vehicle, Subst.vehicle]
+  apply Fintype.image_in_of_all_in
+  intro a h
+  apply Fintype.included_trans _
+    <| Fintype.included_without_of_included _
+    <| Fintype.in_image_of_is_image h
+  apply Fintype.not_mem_iff_in_without.1
+  apply vanishing_on_term h₁ h₂
+
+theorem vanishing_respects_vehicle {θ : Subst α β} (h₁ : vanishing θ) {x : β}
+  (h₂ : ¬ x ∈ (𝒱 θ : Fintype β)) {u : Term α β} (h₃ : ¬ x ∈ (𝒱 u : Fintype β)) :
+  ¬ x ∈ (𝒱 (u • θ) : Fintype β) := by
+  apply Fintype.not_mem_of_superset_not_mem (vehicle_on_image Fintype.included_refl _)
+  intro h
+  rw [Fintype.mem_union_iff] at h
+  exact match h with
+  | Or.inl h => h₂ h
+  | Or.inr h => h₃ h
+
+theorem cons_vanishing {θ φ : Subst α β} {l₁ r₁ l₂ r₂ : Term α β}
+  (h₁ : (𝒱 θ : Fintype β) ⊆ 𝒱 l₁ ∪ 𝒱 l₂)
+  (h₂ : (𝒱 φ : Fintype β) ⊆ 𝒱 (r₁ • θ) ∪ 𝒱 (r₂ • θ))
+  (h₃ : vanishing θ) (h₄ : vanishing φ) : vanishing (θ * φ) := by
+  intro x hx y
+  by_cases hθ : (Term.Var x : Term α β) • θ = Term.Var x
+  focus
+    let p := show (Term.Var x : Term α β) • φ ≠ Term.Var x by
+      intro hφ
+      apply hx
+      rw [← RAction.smul_mul, hθ, hφ]
+    rw [← RAction.smul_mul]
+    apply vanishing_on_term h₄ p
+  focus
+    let p := show ¬ x ∈ (𝒱 φ : Fintype β) by
+      apply Fintype.not_mem_of_superset_not_mem h₂
+      intro h
+      rw [Fintype.mem_union_iff] at h
+      exact match h with
+      | Or.inl h => (vanishing_on_term h₃ hθ r₁) h
+      | Or.inr h => (vanishing_on_term h₃ hθ r₂) h
+    rw [← RAction.smul_mul]
+    exact vanishing_respects_vehicle h₄ p (h₃ hθ _)
+
+theorem elementary_vanishing {x : β} {u : Term α β} {h₁ : Term.Var x ≠ u}
+  (h₂ : ¬ x ∈ (𝒱 u : Fintype β)) :
+  vanishing (Subst.elementary h₁ : Subst α β) := by
+  intro z hz t
+  intro h'
+  have p : z = x := by
+    let p := carrier_spec.2 hz
+    rw [elementary_carrier, Fintype.mem_mk_iff] at p
+    simp_all [List.mem]
+  rw [p] at h'
+  by_cases p' : t = x
+  focus
+    rw [p'] at h'
+    rw [Subst.elementary_spec₁] at h'
+    exact h₂ h'
+  focus
+    rw [Subst.elementary_spec₂ _ p'] at h'
+    apply Ne.symm p'
+    simp_all [HasVehicle.vehicle, Term.vehicle, Fintype.mem_mk_iff, List.mem]
+
+end
+
