Flows/Vehicle.lean
@@ -1,0 +1,164 @@
+/-
+Copyright (c) 2021-2022 Julien Marquet. All rights reserved.
+Released under Apache 2.0 license as described in the file LICENSE.
+Authors: Julien Marquet
+-/
+
+import Flows.SolveSets
+import Flows.Term
+import Flows.Subst
+
+open Classical
+
+set_option codegen false
+
+section
+
+variable {α β : Type u}
+
+def Term.vehicle : Term α β → Fintype β
+| Term.Cst _ => ∅
+| Term.Var x => Fintype.mk [x]
+| Term.Cons l r => vehicle l ∪ vehicle r
+
+instance : HasVehicle (Term α β) (Fintype β) where
+  vehicle := Term.vehicle
+
+def Subst.vehicle (θ : Subst α β) : Fintype β := Fintype.image
+  (λ x => 𝒱 ((Term.Var x : Term α β) • θ)) (carrier θ)
+
+instance : HasVehicle (Subst α β) (Fintype β) where
+  vehicle := Subst.vehicle
+
+theorem vehicle_cons {u v : Term α β} : 
+  (𝒱 (Term.Cons u v) : Fintype β) = 𝒱 u ∪ 𝒱 v := rfl
+
+theorem vehicle_one : 𝒱 (1 : Subst α β) = (∅ : Fintype β) := by
+  rw [Fintype.ext]
+  intro x
+  apply Iff.intro _ (λ h => False.elim h)
+  simp only [HasVehicle.vehicle, Subst.vehicle]
+  rw [Fintype.mem_image_iff, carrier_one]
+  intro ⟨ _, p, _ ⟩
+  exact Fintype.not_mem_empty _ p
+
+theorem vehicle_elementary {x : β} {u : Term α β} (h : Term.Var x ≠ u) :
+  𝒱 (Subst.elementary h : Subst α β) = (𝒱 u : Fintype β) := by
+  apply Fintype.ext.2
+  intro z
+  apply Iff.intro
+  focus
+    intro h'
+    simp only [HasVehicle.vehicle, Subst.vehicle] at h'
+    let ⟨ t, t_in, in_img ⟩ := Fintype.mem_image_iff.1 h'
+    rw [elementary_carrier, Fintype.mem_mk_iff] at t_in
+    rw [show t = x by simp_all [List.mem],
+      Subst.elementary_spec₁] at in_img
+    exact in_img
+  focus
+    intro p
+    simp only [HasVehicle.vehicle, Subst.vehicle]
+    apply Fintype.mem_image_iff.2 ⟨ x, (show x ∈ carrier _ from _), _ ⟩
+    focus
+      rw [elementary_carrier, Fintype.mem_mk_iff]
+      simp [List.mem]
+    focus
+      rw [Subst.elementary_spec₁]
+      exact p
+
+theorem vehicle_on_image {θ : Subst α β} {A : Fintype β}
+  (h₁ : 𝒱 θ ⊆ A) (u : Term α β) :
+  𝒱 (u • θ) ⊆ A ∪ 𝒱 u := by
+    induction u with
+    | Cst c => cases θ; apply Fintype.empty_included
+    | Var x =>
+      by_cases h : (Term.Var x : Term α β) • θ = Term.Var x
+      focus
+        apply Fintype.included_union_l
+        rw [h]
+        exact Fintype.included_refl
+      focus
+        apply Fintype.included_union_r
+        apply Fintype.included_trans _ h₁
+        intro y h'
+        apply Fintype.in_image_of_is_image <| carrier_spec.2 h
+        exact h'
+    | Cons l r hl hr =>
+      rw [subst_cons]
+      simp only [Term.vehicle]
+      apply Fintype.included_trans (Fintype.union_on_included hl hr)
+      rw [vehicle_cons]
+      solve_sets
+
+theorem vehicle_on_image_contained {θ : Subst α β} {A : Fintype β} {u : Term α β}
+  (h₁ : 𝒱 θ ⊆ A) (h₂ : 𝒱 u ⊆ A) : 𝒱 (u • θ) ⊆ A :=
+  Fintype.included_trans (vehicle_on_image h₁ u) <|
+    Fintype.union_included_iff.2 ⟨ Fintype.included_refl, h₂ ⟩
+
+theorem vehicle_on_comp {θ φ : Subst α β} {A : Fintype β}
+  (h₁ : 𝒱 θ ⊆ A) (h₂ : 𝒱 φ ⊆ A) : 𝒱 (θ * φ) ⊆ A := by
+  simp only [HasVehicle.vehicle, Subst.vehicle]
+  apply Fintype.image_in_of_all_in
+  intro x h
+  rw [carrier_spec] at h
+  simp only [] -- Better way to do it ?
+  rw [← RAction.smul_mul]
+  by_cases hθ : (Term.Var x : Term α β) • θ = Term.Var x
+  focus
+    have hφ := show (Term.Var x : Term α β) • φ ≠ Term.Var x by
+      intro hφ
+      apply h
+      rw [← RAction.smul_mul, hθ, hφ]
+    rw [hθ]
+    apply Fintype.included_trans _ h₂
+    intro y h'
+    apply Fintype.in_image_of_is_image <| carrier_spec.2 hφ
+    exact h'
+  focus
+    apply vehicle_on_image_contained h₂
+    -- The pattern of the four following lines occurs often.
+    -- Make it a lemma ?
+    apply Fintype.included_trans _ h₁
+    intro y h'
+    apply Fintype.in_image_of_is_image <| carrier_spec.2 hθ
+    exact h'
+
+theorem vehicle_on_comp₁ (θ φ : Subst α β) : 
+  (𝒱 (θ * φ) : Fintype β) ⊆ 𝒱 θ ∪ 𝒱 φ := vehicle_on_comp
+  (Fintype.included_union_r _ <| Fintype.included_refl)
+  (Fintype.included_union_l _ <| Fintype.included_refl)
+
+theorem cons_vehicle_in {θ φ : Subst α β} {l₁ r₁ l₂ r₂ : Term α β}
+  (h₁ : (𝒱 θ : Fintype β) ⊆ 𝒱 l₁ ∪ 𝒱 l₂)
+  (h₂ : (𝒱 φ : Fintype β) ⊆ 𝒱 (r₁ • θ) ∪ 𝒱 (r₂ • θ)) :
+  (𝒱 (θ * φ) : Fintype β) ⊆ 𝒱 (Term.Cons l₁ r₁) ∪ 𝒱 (Term.Cons l₂ r₂) := by
+  rw [vehicle_cons, vehicle_cons]
+  apply Fintype.included_trans (vehicle_on_comp₁ θ φ)
+  rw [Fintype.union_included_iff]; apply And.intro
+  focus
+    apply Fintype.included_trans h₁
+    solve_sets
+  focus
+    apply Fintype.included_trans h₂
+    apply Fintype.union_included_iff.2 ⟨ _, _ ⟩
+      <;> apply vehicle_on_image_contained
+      <;> try apply Fintype.included_trans h₁
+    all_goals solve_sets
+
+theorem elementary_on_not_in_vehicle {x : β} {u v : Term α β} (h : Term.Var x ≠ u)
+  (h' : ¬ x ∈ (𝒱 v : Fintype β)) :
+  v • (Subst.elementary h : Subst α β) = v := by
+  induction v with
+  | Cst c => rfl
+  | Var y =>
+    apply Subst.elementary_spec₂
+    intro h
+    apply h'
+    rw [h]
+    simp [HasVehicle.vehicle, Term.vehicle, Fintype.mem_mk_iff, List.mem]
+  | Cons l r hl hr =>
+    rw [vehicle_cons, Fintype.mem_union_iff] at h'
+    rw [subst_cons, hl (λ h => h' <| Or.inl h), hr (λ h => h' <| Or.inr h)]
+
+end
+
